RocqOfRust/revm/revm_interpreter/instructions/links/bitwise/clz.v
@@ -1,0 +1,41 @@
+Require Import RocqOfRust.RocqOfRust.
+Require Import links.RocqOfRust.
+Require Import core.convert.links.num.
+Require Import core.links.cmp.
+Require Import core.links.option.
+Require Import core.links.result.
+Require Import core.num.links.error.
+Require Import core.num.links.mod.
+Require Import revm.revm_interpreter.gas.links.constants.
+Require Import revm.revm_interpreter.links.gas.
+Require Import revm.revm_interpreter.links.instruction_context.
+Require Import revm.revm_interpreter.links.instruction_result.
+Require Import revm.revm_interpreter.links.interpreter.
+Require Import revm.revm_interpreter.links.interpreter_types.
+Require Import revm.revm_interpreter.instructions.bitwise.
+Require Import revm.revm_primitives.links.hardfork.
+Require Import ruint.links.bits.
+Require Import ruint.links.cmp.
+Require Import ruint.links.from.
+Require Import ruint.links.lib.
+
+Instance run_bitwise_clz
+    {WIRE H : Set} `{Link WIRE} `{Link H}
+    {WIRE_types : InterpreterTypes.Types.t} `{InterpreterTypes.Types.AreLinks WIRE_types}
+    (run_InterpreterTypes_for_WIRE : InterpreterTypes.Run WIRE WIRE_types)
+    (context : InstructionContext.t H WIRE WIRE_types) :
+  Run.Trait
+    instructions.bitwise.clz [] [ Φ WIRE; Φ H ] [ φ context ]
+    unit.
+Proof.
+  constructor.
+  destruct run_InterpreterTypes_for_WIRE eqn:?.
+  destruct run_StackTrait_for_Stack.
+  destruct run_LoopControl_for_Control.
+  destruct run_RuntimeFlag_for_RuntimeFlag.
+  destruct (TryFrom_usize_for_Uint.run {| Integer.value := 256 |} {| Integer.value := 4 |}).
+  run_symbolic.
+  { eapply Impl_Interpreter.run_halt_not_activated. }
+  { eapply Impl_Interpreter.run_halt_underflow. }
+Defined.
+Global Opaque run_bitwise_clz.
