RocqOfRust/revm/revm_interpreter/instructions/simulate/bitwise/clz.v
@@ -1,0 +1,86 @@
+Require Import simulate.RocqOfRust.
+Require Import alloy_primitives.links.aliases.
+Require Import core.links.array.
+Require Import core.links.cmp.
+Require Import core.simulate.cmp.
+Require Import core.simulate.option.
+Require Import revm.revm_context_interface.links.host.
+Require Import revm.revm_interpreter.gas.simulate.constants.
+Require Import revm.revm_interpreter.instructions.links.bitwise.clz.
+Require Import revm.revm_interpreter.instructions.simulate.macros.
+Require Import revm.revm_interpreter.links.instruction_context.
+Require Import revm.revm_interpreter.links.interpreter.
+Require Import revm.revm_interpreter.links.interpreter_types.
+Require Import revm.revm_interpreter.simulate.interpreter_types.
+Require Import revm.revm_primitives.links.hardfork.
+Require Import revm.revm_primitives.simulate.hardfork.
+Require Import ruint.links.lib.
+Require Import ruint.simulate.bits.
+Require Import ruint.simulate.cmp.
+Require Import ruint.simulate.from.
+
+Definition op_clz
+    {WIRE : Set} `{Link WIRE}
+    {WIRE_types : InterpreterTypes.Types.t} `{InterpreterTypes.Types.AreLinks WIRE_types}
+    {IInterpreterTypes : InterpreterTypes.C WIRE_types}
+    (interpreter : Interpreter.t WIRE WIRE_types) :
+    Interpreter.t WIRE WIRE_types :=
+  check_macro interpreter SpecId.OSAKA id (fun interpreter =>
+  popn_top_macro interpreter 0 id (fun arr top interpreter =>
+    let op1 := top.(RefStub.projection) interpreter.(Interpreter.stack) in
+    let leading_zeros := Impl_Uint.leading_zeros op1 in
+    let result : aliases.U256.t := Impl_Uint.from leading_zeros in
+    let stack :=
+      top.(RefStub.injection)
+        interpreter.(Interpreter.stack) result in
+    interpreter
+      <| Interpreter.stack := stack |>
+  )).
+
+Lemma op_clz_eq
+    {WIRE H : Set} `{Link WIRE} `{Link H}
+    {WIRE_types : InterpreterTypes.Types.t} `{InterpreterTypes.Types.AreLinks WIRE_types}
+    {H_types : Host.Types.t} `{Host.Types.AreLinks H_types}
+    (run_InterpreterTypes_for_WIRE : InterpreterTypes.Run WIRE WIRE_types)
+    (IInterpreterTypes : InterpreterTypes.C WIRE_types)
+    (InterpreterTypesEq :
+      InterpreterTypes.Eq.t WIRE WIRE_types run_InterpreterTypes_for_WIRE IInterpreterTypes)
+    (interpreter : Interpreter.t WIRE WIRE_types)
+    (_host : H) :
+  let ref_interpreter : '&mut (Interpreter.t WIRE WIRE_types) := make_ref 0 in
+  let ref_host : '&mut H := make_ref 1 in
+  let context := {|
+    instruction_context.InstructionContext.interpreter := ref_interpreter;
+    instruction_context.InstructionContext.host := ref_host;
+  |} in
+  {{
+    SimulateM.eval_f
+      (run_bitwise_clz run_InterpreterTypes_for_WIRE context)
+      ([interpreter; _host]%stack) 🌲
+    (
+      Output.Success tt,
+      [
+        op_clz interpreter;
+        _host
+      ]%stack
+    )
+  }}.
+Proof.
+  intros.
+  unfold op_clz.
+  check_macro_eq InterpreterTypesEq.
+  popn_top_macro_eq InterpreterTypesEq.
+  eapply Run.Call; [
+    eapply Impl_Option.unwrap_unchecked_eq;
+    reflexivity
+  |].
+  cbn.
+  lu.
+  s. {
+    apply Impl_Uint.leading_zeros_eq; repeat unshelve econstructor.
+  }
+  s. {
+    apply Impl_Uint.from_eq; [typeclasses eauto | easy].
+  }
+  s.
+Qed.
